### Idea
- Let $\oplus$ denote the `XOR` operation, $+$ denote the `OR` operation, and $.$ denote the `AND` operation.
- Consider $n$ elements $A_1, A_2, A_3, ..., A_n$.
- We create the following table, where the `OR` sums in the column of element $A_i$ start from ${1, 2, ..., i - 1, i}$ and end at $i$. These are also the sums needed to compute the `XOR` total.

| Element $A_1$ | Element $A_2$ | Element $A_3$ | ... | Element $A_n$ |
|:-------------:|:-------------:|:-------------:|:---:|:-------------:|
| $f(1, 1)$     | $f(1, 2)$     | $f(1, 3)$     | ... | $f(1, n)$     |
|               | $f(2, 2)$     | $f(2, 3)$     | ... | $f(2, n)$     |
|               |               | $f(3, 3)$     | ... | $f(3, n)$     |
|               |               |               | ... |      ...      |
|               |               |               | ... | $f(n, n)$     |
| _____________ | _____________ | _____________ | ___ | _____________ |
| $F(1, 1)$     | $F(1, 2)$     | $F(1, 3)$     | ... | $F(1, n)$     |

- Define $F(1, k)$ as the `XOR` sum of the `OR` sums ending at $k$.
- Therefore, the problem becomes: Compute the `XOR` sum of all $F(1, k)$ for $k \in \{1, 2, ..., n\}$.
- We have: $F(1, 1) = f(1, 1) = A_1$.
- Next: $F(1, 2) = f(1, 2) \oplus f(2, 2) = (A_1 + A_2) \oplus (A_2) = A_1.\overline{A_2}$.
- Next: $F(1, 3) = f(1, 3) \oplus f(2, 3) \oplus f(3, 3) = (A_1 + A_2 + A_3) \oplus (A_2 + A_3) \oplus (A_3) = A_1.\overline{A_2} + A_3$.
- Next: $F(1, 4) = (A_1.\overline{A_2} + A_3).\overline{A_4}$.

- Using mathematical induction, we can derive the following recurrence formula:
$$ 
F(1, n) = 
\begin{cases} 
A_1, &\text{if } n == 1 \newline
F(1, n - 1) + A_n, & \text{if } n\text{ is odd} \newline 
F(1, n - 1).\overline{A_n} , & \text{if } n\text{ is even} 
\end{cases} 
$$

### C++ Code
```cpp
// nxxhoang - the dreamer
#include <bits/stdc++.h>
#define FOR(i, a, b) for (int i = a; i < (int)b; i++)
#define endl '\n'

using namespace std;
using ll = long long;
using ull = unsigned long long;

void solve(){
    int n, a, result = 0, cur = 0;
    cin >> n;
    FOR (i, 1, n + 1) {
        cin >> a;
        if (i % 2) cur |= a;
        else cur &= ~a;
        result ^= cur;
    }
    cout << result;
}

int main()
{
    ios_base::sync_with_stdio(false);
    cin.tie(NULL);
    cout.tie(NULL);
    solve();
    return 0;
}
```
